Test/git-issues/git-issue-697h.dfy
@@ -5,6 +5,13 @@ ghost const maxi := 4;
 
 type substring = x: string | |x| < maxi
 
+method firstParameterGhost(ghost b: bool, i: int) {
+}
+
+function method firstParameterGhostFun(ghost b: bool): int {
+  2
+}
+
 // It's ok to have not compiled subset types in all specification expressions
 method test(s: seq<substring>) returns (r: int)
   requires forall x: substring :: x in s ==> |x| < maxi
@@ -16,6 +23,15 @@ method test(s: seq<substring>) returns (r: int)
     r := j;
   }
   assert forall x: substring :: x in s ==> |x| < maxi;
+  ghost var z := true;
+  if z {
+    var w := forall x: substring :: x in s ==> |x| < maxi;
+  }
+  firstParameterGhost(forall x: substring :: x in s ==> |x| < maxi,
+    firstParameterGhostFun(forall x: substring :: x in s ==> |x| < maxi)
+  );
+  var x := firstParameterGhostFun(forall x: substring :: x in s ==> |x| < maxi);
+  var h := forall x: substring :: x in s ==> |x| < maxi;
   while true
     invariant forall x: substring :: x in s ==> |x| < maxi
   {
